Work on rule graphs

coq/lang/RuleGraphs.v
@@ -1,5 +1,127 @@
 Set Implicit Arguments.
-From Lang Require Export Assertions.
+From Lang Require Export Util.
+From Coq Require Import Structures.OrderedTypeEx.
+From Coq Require FSetList FSetFacts.
+
+Variable stmt : Type.
+Variable liftable : stmt -> Prop.
+Variable valid_stmt : stmt -> Prop.
+
+Variable rule : Type.
+Variable valid_rule : rule -> list stmt -> stmt -> Prop.
+
+Definition sound_rule (r : rule) : Prop :=
+  forall (prems : list stmt) (conc : stmt),
+    valid_rule r prems conc ->
+      LibList.Forall valid_stmt prems ->
+      valid_stmt conc.  
+
+Module Node <: UsualOrderedType.
+  Include Nat_as_OT.
+End Node.
+
+Notation node := Node.t.
+
+Module Import NodeSet := FSetList.Make(Node).
+Module NodeSetFacts := FSetFacts.Facts(NodeSet).
+
+Variant rule_or_lift : Type :=
+  | Rule (r : rule) 
+  | Lift.
+
+Inductive rule_graph : Type := {
+  rg_nodes : NodeSet.t;
+  rg_node  : Type := {nd | NodeSet.mem nd rg_nodes};
+  rg_conc  : rg_node -> stmt;
+  rg_rule  : rg_node -> rule_or_lift;
+  rg_prems : rg_node -> list rg_node;
+  rg_wf    : forall nd : rg_node, 
+              match rg_rule nd with
+              | Rule r => valid_rule r (List.map rg_conc (rg_prems nd)) (rg_conc nd)
+              | Lift => liftable (rg_conc nd) /\ (rg_prems nd) = nil
+              end
+}.
+
+Section RuleGraph.
+
+Variable rg : rule_graph.
+
+Notation rg_node := rg.(rg_node).
+
+Definition valid_rule_graph : Prop :=
+  forall (nd : rg_node), 
+    match rg_rule nd with
+    | Lift => valid_stmt (rg_conc nd)
+    | _ => True
+    end.
+
+Fixpoint is_path (p : list rg_node) : Prop :=
+  match p with
+  | nd1 :: p => 
+    match p with 
+    | nd2 :: p' => List.In nd2 (rg_prems nd1) /\ is_path p
+    | _ => True
+    end
+  | _ => True
+  end.
+
+Definition path : Type := 
+  {p : list rg_node | is_path p}.
+
+(* Fixpoint path_end (nd : rg_node) (p : list rg_node) : Prop :=
+  match p with
+  | [] => False
+  | nd1 :: [] => nd1 = nd
+  | nd1 :: p => path_end nd p
+  end. *)
+
+Definition ne_list : list int := [5].
+Lemma ne_easy : ne_list <> [].
+  discriminate.
+Qed.
+
+Definition reaches (nd1 nd2 : rg_node) : Prop :=
+  exists (p : path),
+    match classicT (proj1_sig p <> []) with
+    | left H => ListFacts.get_nonempty_first H = nd1 /\ ListFacts.get_nonempty_last H = nd2
+    | _ => False
+    end.
+
+Lemma reaches_refl nd : reaches nd nd.
+  unfolds.
+  assert (is_path (nd :: nil)) by (now unfold is_path). 
+  exists (exist _ _ H).
+  destruct (classicT (proj1_sig (exist is_path [nd]%list H) <> [])).
+  simpls.
+  + split.
+    - unfold get_nonempty_first.
+      destruct (constructive_definite_description _ _).
+      simpl.
+      unfold first in e.
+      injects e.
+      reflexivity.
+    - unfold get_nonempty_last.
+      destruct (constructive_definite_description _ _).
+      simpl.
+      unfold last in e.
+      injects e.
+      reflexivity.
+  + simpls. 
+    contradict n.
+    discriminate.
+Qed.
+
+End RuleGraph.
+
+
+
+
+
+
+
+(* 
+
+
 
 Implicit Type m : mem.
 Implicit Type n : int.
@@ -341,4 +463,4 @@ Proof.
 Abort.
 
 
-End Soundness.
+End Soundness. *)
